\documentclass[11pt]{article} 



\makeatletter
\renewcommand\section{\@startsection{section}{1}{\z@}%
                                  {-3.5ex \@plus -1ex \@minus -.2ex}%
                                  {2.3ex \@plus.2ex}%
                                  {\normalfont\large\bfseries}}
\makeatother

\addtolength{\oddsidemargin}{-.875in}
\addtolength{\evensidemargin}{-.875in}
\addtolength{\textwidth}{1.75in}
\addtolength{\topmargin}{-.875in}
\addtolength{\textheight}{1.75in}


\usepackage{amssymb}
\usepackage{amsmath}
\usepackage{amsthm}
\usepackage{graphicx,caption,subcaption}


\usepackage{titling}
\setlength{\droptitle}{-6em}
\posttitle{\par\end{center}\vspace{-4.8em}}

\newcommand{\R}{{\ensuremath{\mathbb{R}}} }
\newcommand{\Q}{{\ensuremath{\mathbb{Q}}} }
\newcommand{\C}{{\ensuremath{\mathbb{C}}} }
\newcommand{\N}{{\ensuremath{\mathbb{N}}} }
\newcommand{\Z}{{\ensuremath{\mathbb{Z}}} }

\newcommand{\sexion}{\addtocounter{section}{1} }


\newcommand{\hint}[1]{{(\emph{Hint:} #1)}} %This line shows hints
%\newcommand{\hint}[1]{} %Use this line to hide all hints


\usepackage{fancyhdr}
\pagestyle{fancyplain}
\renewcommand{\headrulewidth}{0pt}

\begin{document}

%\lhead{}
\rhead{Complex System}

We solve 
\[\vec{y'} = A \vec{y}\quad\mathrm{for}\quad A = \left(
\begin{array}{cc}
 0 & 4 \\
 -2 & -4
\end{array}
\right) \quad\mathrm{satisfying}\quad y(0) = \left( \begin{matrix} 0 \\-1 \end{matrix} \right) \]

First, compute the characteristic polynomial
\[|A - \lambda I | = \lambda ^2+4 \lambda +8\]
and use the quadratic equation to find the roots $ \lambda =  -2+2 i $ and $ \bar{\lambda} = -2-2 i$. Now we must find an eigenvector corresponding to each eigenvalue. If $v$ is an eigenvector for $\lambda$, then $\bar{v}$ is an eigenvector for $\bar{\lambda}$, so we can just compute 
\[A \left( \begin{matrix} v_1 \\ v_2 \end{matrix} \right) = \lambda  \left( \begin{matrix} v_1 \\ v_2 \end{matrix} \right) \iff \begin{matrix} 4 v_2 = (-2 + 2i) v_1 \\ -2 v_1 -4 v_2 = (-2+2i) v_2 \end{matrix}  \iff \begin{matrix} (2 - 2i) v_1 + 4 v_2=0 \\ -2 v_1  +(-2-2i) v_2 =0\end{matrix} \]
but since $\lambda = -2 + i$ is an eigenvalue, these two equations are equivalent. This may be a bit hard to see because of the complex numbers, so let's check:
\[\left(-\frac{1}{2} - \frac{i}{2}\right) \left((2 - 2i) v_1 + 4 v_2 \right)  =
\left(-\frac{1}{2} - \frac{i}{2}\right) (2 - 2i) v_1 + 4 \left(-\frac{1}{2} - \frac{i}{2}\right)  v_2   = -2 v_1  +(-2-2i) v_2 =0  \]
Now all we have to do is come up with some eigenvector which satisfies one (both) of these equations. Let's choose 
\[v = \left(
\begin{array}{c}
 -1-i \\
 1
\end{array}
\right)\]

Recall that the general solution to this sort of equation is given by 
\[ y = C_1 e^{\lambda t} v + C_2 e^{\bar{\lambda} t } \bar{v} \leadsto  C_1 e^{(-2 + 2i)t}  \left( \begin{matrix} -1-i \\ 1 \end{matrix} \right) + C_2 e^{(-2 - 2i)t}  \left( \begin{matrix} -1+i \\1 \end{matrix} \right)\]
So, in order to satisfy our initial conditions, we must have
\[ y(0) =  C_1   \left( \begin{matrix} -1-i \\ 1 \end{matrix} \right) + C_2  \left( \begin{matrix} -1+i \\1 \end{matrix} \right) =  \left( \begin{matrix} 0 \\-1 \end{matrix} \right) \]
so, $C_1 =  -\frac{1}{2}-\frac{i}{2},C_2 =  -\frac{1}{2}+\frac{i}{2}$. Therefore, the solution is just
\[ \left(-\frac{1}{2}-\frac{i}{2} \right) e^{(-2 + 2i)t}  \left( \begin{matrix} -1-i \\ 1 \end{matrix} \right) + \left( -\frac{1}{2}+\frac{i}{2}\right) e^{(-2 - 2i)t}  \left( \begin{matrix} -1+i \\1 \end{matrix} \right)\]
Let's find the real part
\begin{align*}
y &= \Re \left[ \left(-\frac{1}{2}-\frac{i}{2} \right) e^{(-2 + 2i)t}  \left( \begin{matrix} -1-i \\ 1 \end{matrix} \right) + \left( -\frac{1}{2}+\frac{i}{2}\right) e^{(-2 - 2i)t}  \left( \begin{matrix} -1+i \\1 \end{matrix} \right) \right]\\
&= e^{-2t} \Re \left[ \left(-\frac{1}{2}-\frac{i}{2} \right) e^{ 2it}  \left( \begin{matrix} -1-i \\ 1 \end{matrix} \right) + \left( -\frac{1}{2}+\frac{i}{2}\right) e^{- 2it}  \left( \begin{matrix} -1+i \\1 \end{matrix} \right) \right]\\
&= e^{-2t} \Re \left[  e^{ 2it}  \left( \begin{matrix} \left(-\frac{1}{2}-\frac{i}{2} \right)(-1-i) \\ -\frac{1}{2}-\frac{i}{2} \end{matrix} \right) +  e^{- 2it}  \left( \begin{matrix}\left( -\frac{1}{2}+\frac{i}{2}\right)( -1+i) \\  -\frac{1}{2}+\frac{i}{2} \end{matrix} \right) \right]\\
&= e^{-2t} \Re \left[ (\cos 2t + i \sin 2t ) \left( \begin{matrix} i\\ -\frac{1}{2}-\frac{i}{2} \end{matrix} \right) +  (\cos(-2t) + i \sin(-2t))  \left( \begin{matrix} -i \\  -\frac{1}{2}+\frac{i}{2} \end{matrix} \right) \right]\\
&= e^{-2t} \left(  \left( \begin{matrix} -\sin 2t\\ -\frac{1}{2}\cos 2t +\frac{1}{2} \sin 2t \end{matrix} \right) +   \left( \begin{matrix}\sin(-2t)  \\  -\frac{1}{2} \cos(-2t) -\frac{1}{2} \sin(-2t) \end{matrix} \right) \right) \\
&= e^{-2t}  \left( \begin{matrix} -2 \sin 2t \\ -\cos 2t + \sin 2t \end{matrix} \right)  \\
\end{align*}




\end{document}
