\documentclass[14pt]{article}

\usepackage{amsthm, amsmath, graphicx, hyperref} 

\usepackage[margin=1in]{geometry}

\title{33B: Notes}
\author{Frederick Robinson}

\newtheorem{defn}{Definition}
\newtheorem{re}{Recipe}
\newtheorem{ex}{Example}
\newtheorem{thm}{Theorem}

\newcommand{\type}[1]{\begin{center} \emph{\textbf{#1}} \end{center}}
\newcommand{\exs}{\subsubsection*{Examples}}



\begin{document}

\maketitle
\tableofcontents
\pagebreak

Frederick Robinson

frobinson@math.ucla.edu

math.ucla.edu/$\sim$frobinson

Office Hours: ----- (or by appointment)
MS 3969

\section*{Format}

Generally I'll spend the first part (at most $1/2$) of class on exposition, recapping the material
from class. The rest of class will be spent on working examples similar to those on your homework. 

\pagebreak

\section{Introduction}

Differential equations are just equations involving the derivatives of functions. There are partial
differential equations - differential equations involving partial derivatives of functions, and
ordinary differential equations - differential equations which just involve ordinary derivatives. 

We can also classify differential equations by the order of the derivatives they involve:
\begin{defn}[Order]The \emph{order} of a differential equation is just the order of the highest
  order derivative that it involves.\end{defn}

Differential equations don't specify just one solution, but rather a family of solutions. For
instance consider $x' = 3$. This equation is solved by $x = 3t$ and $x = 3t + 5$. In general
solutions are exactly those equations of the form $x = 3t + C$. We call this the \emph{general
  solution}.

\begin{defn}[General Solution]
  The \emph{general solution} to an ordinary differential equation of order $n$ is an equation
  containing $n$ constants which describes all possible solutions to the equation. 
\end{defn}

Often we're interested in one particular solution to a differential equation which satisfies
constraints of the form $y^{(n)}(t) = y_0$. We call these constraints \emph{initial
  conditions}. This sort of problem is called an \emph{initial value problem}. It takes $n$
conditions to fully specify a \emph{particular solution} to a differential equation of order $n$.

Suppose in our example above that in addition to the differential equation $x'=3$ we had specified
that $x(5) = 4$, then we could find a particular solution by first finding the general solution $x =
3t + C$, and then plugging in the initial condition: $x(5) = 3 \cdot 5 + C = 4 \Rightarrow C =
-1$. Our solution is then just $x(t) = 3 t -1 $.


\subsection*{Examples}
Give some examples of PDE / ODEs of different orders...

Differential equations come up all the time in practical applications. Here's a really simple
example problem. 

\begin{ex}
  A ball is dropped from a height of 100m. It's position as a function of time satisfies the (second
  order linear) differential equation
  \[\frac{d^2x}{dt^2} = -10 m/s^2 \]
  When does it hit the ground?
\end{ex}

We should be able to solve this without any new techniques. Just integrate.
  \[\frac{d^2x}{dt^2} = -10 m/s^2 \Rightarrow \frac{dx}{dt} = -10 t + C \Rightarrow x(t) = -5 t^2 +
  C t + D \] Of course, this doesn't really specify the location of our ball. We need to use our
  initial conditions. Since we dropped ball, initial acceleration is $x'(0) = 0$, also we are given
  $x(0) = 100$. Substituting these into general solution we have:
  \[x'(0) = -10 t + C = C = 0\] and
  \[x(0) = -5 t^2 + C t + D = D = 100.\]

Thus, solve
\[0 = x(t) = -5 t^2 + 100 \Rightarrow t = \pm \sqrt{20}.\]
Clearly our solution must be positive, so the answer is $2 \sqrt 5$ seconds.

Of course this is a sort of silly example since we can solve it by integration. We'll solve harder
problems later using more sophisticated techniques.

\section{Chapter 2}

\subsection{Section 1}

If we have a purported solution $y(t)$ to some differential equation, we can check that it's
actually valid by differentiating and checking to see that the derivatives satisfy whatever equation
they are supposed to satisfy.

\begin{defn}[Interval of Existence]
  The \emph{interval of existence} for an initial value problem is the largest interval on which a
  solution exists and satisfies the differential equation.
\end{defn}

For instance, the interval of existence for $x' =3; x(0)=0$ is $(-\infty, \infty)$ since the
solution $x = 3t$ exists, and satisfies the given differential equation for all time.


\begin{defn}[Normal form]
  An order $n$ differential equation is said to be in \emph{normal form} if it is of the form $y^{(n)} = f(y^{(n-1)}, y^{(n-2)}, \dots, y',y,t)$.
\end{defn}

Given a first order ODE in normal form $y' = f(y,t)$ we can draw a vector field describing solutions
by drawing small lines of slope $f(y,t)$ at some collection of points $(y,t)$.

\exs

\type{Check}
\begin{ex}[Exercise 2.1.3] Check that $y' = -ty$ is solved by $y = C e ^{-(1/2) t^2}$\end{ex}

Just differentiate and compare:
\[y' = -t C e^{-(1/2) t^2} = -t y\]
so it is a solution to the differential equation.

\type{Interval of Existence}
\begin{ex}[Exercise 2.1.13] Find the interval of existence for the differential equation $y' =
  \frac{2}{3} t - \frac{5}{3 t^2}  $ satisfying initial condition $y(1) = 2$ \end{ex}

We can solve by integration:
\begin{align*}
\frac{dy}{dt}  &= \frac{2}{3} t - \frac{5}{3 t^2}\\
dy &= \left( \frac{2}{3} t - \frac{5}{3 t^2} \right) dt\\
y &= \frac{1}{3} t^2 + \frac{5}{3t} + C
\end{align*}
This is the general solution. If we further demand $y(1) = 2$
\[y(1) = \frac{1}{3} + \frac{5}{3} + C = 2 \Rightarrow C = 0\]
Therefore
\[y(t) = \frac{1}{3} t^2 + \frac{5}{3 t} \]
is the particular solution we're after.

Now that we have the solution it's easy to determine interval of existence. There's an asymptote at
$t=0$, so that is the lower end of the interval. The function is continuous as $t \to \infty$, so
there is no upper limit. Interval of existence is therefore $(0,\infty)$.

\type{Normal Form}
\begin{ex}[Exercise 2.1.1] Put $\phi(t,y,y') = t^2 y' + (1+t) y = 0$ in normal form. \end{ex}
Just solve for $y'$: 
\[y' = - \frac{y(1+t)}{t^2} \]


\type{Vector Field}
\begin{samepage}
\begin{ex}[Exercise 2.1.17] Draw vector field for $y' = y+ t$. \end{ex}
\[\includegraphics[scale=.7]{figures/{2.1.17}.pdf}\]
\end{samepage}

\begin{samepage}
\begin{ex}[Exercise 2.1.19] Draw vector field for $y' = t \tan{y/2}$. \end{ex}
\[\includegraphics[scale=.7]{figures/{2.1.19}.pdf}\]
\end{samepage}

\pagebreak

\begin{samepage}
\begin{ex}[Exercise 2.1.19] Draw vector field for $y' = \frac{x-y}{x+y}$. \end{ex}
\[\includegraphics[scale=.7]{figures/{2.1.extra}.pdf}\]
\end{samepage}

\subsection{Section 2 - Separation of Variables}

\exs

\begin{ex}[2.2.5] Find the general solution for $y' = y(x+1)$. \end{ex}

\[y = C e^{1/2 x^ 2 + x }\]

\begin{ex}[2.2.13] Find the exact solution to the IVP. Indicate interval of existence $ \frac{dy}{dx} = y/x$; $y(1) = -2$. \end{ex}

$y = -2x$, $x \in (0, \infty)$ since DE undefined at $x = 0$.


\begin{ex}[2.2.15] Find the exact solution to the IVP. Indicate interval of existence $ \frac{dy}{dx} = \frac{\sin x}{y}$; $y(\pi / 2 ) = 1$.\end{ex}

\begin{align*}
ydy &= \sin x dx \\
1/2 y^2 &= -\cos x + C \\
y^2 &= -2 \cos x + C \\
y &= \pm \sqrt{-2 \cos x + C } \\ 
\end{align*}

initial condition means that 
\[y(\pi /2 )  = 1 = \sqrt{-2 \cos \pi / 2 + C}\]
so $C =1$ and the solution is 
\[y = \sqrt{1 - 2 \cos x}.\]
The interval of existence is 
\[2 \cos x < 1 \Leftrightarrow \pi / 3 < x < 5 \pi /3 .\]
There is no equality because original equation is undefined.

\addtocounter{subsection}{1}
\subsection{Section 4 - Linear Equations}

\begin{defn}[Linear Homogeneous] A \emph{linear homogeneous} differential equation is one of the form \[x'(t) = a(t) x(t) \] for some function $a(t)$. \end{defn}

We can solve these by separation of variables:
\begin{align*} 
\frac{1}{x} dx &= a(t) dt \\ 
\ln x &= \int a(t) dt + C \\
x &= C e^{\int a(t) dt}
\end{align*}

\begin{defn}[Linear Inhomogeneous] A \emph{linear inhomogeneous} differential equation is one of the form \[x'(t) = f(t) x(t) + g(t) \] for some functions $f(t), g(t)$. \end{defn}

We have two main techniques for solving these: Integrating Factor, and Variation of Parameter.

\begin{re} Integrating Factor:
\begin{enumerate} 
\item Write $x' - ax = f$.
\item Multiply by $u(t) = e^{- \int a(t) dt}$ to get $ (u x)' = uf $.
\item Integrate to get $u(t) x(t) = \int u(t) f(t) dt + C $.
\item Solve for $x$. 
\end{enumerate}
\end{re}

\begin{re} Variation of Parameter:
\begin{enumerate}
\item Put $y' = a y + f $, and solve  associated homogeneous equation $ y'_{hom} = a y_{hom}$.
\item Substitute guess $y = v(t) y_{hom}$ into original equation and solve for $v$. 
\item Write general solution $y = v(t) y_{hom}$.
\end{enumerate}
\end{re}

\exs

\type{Variation of Parameter}

\begin{ex} Solve $y' -2 y = t^2 e^{2 t  }$ by variation of paramenter.\end{ex}

First solve the associated homogeneous: $y'_{hom} = 2 y_{hom}$.
\begin{align*} \frac{1}{y} dy &= 2 dt \\
ln y &= 2 t + C \\
y_{hom} &= C e^{2t}
\end{align*}

Now we `guess' $ y = v(t) y_{hom}$. Since $y' = v' y_{hom} + v y'_{hom} = v' e^{2t} + 2  v e^{2t}$ we have:
\[v' e^{2t} + 2  v e^{2t} - 2(v e^{2t}) = t^2 e^{2t} \Rightarrow v' = t^2 \Rightarrow v = \frac{1}{3} t^3 + C\]
Therefore, $y = e^{2t} \left( \frac{1}{3} t^3 + C \right)$.

\begin{ex}\label{vopint} Solve  $y' + y / t = 3 \cos{(2t)}$ by variation of parameter.\end{ex}

First solve $y_{hom}  + y_{hom} / t = 0$
\begin{align*} \int \frac{1}{y} dy &= - \int \frac{1}{t} dt \\ y_{hom} &= C / t\end{align*}
So put $y = v(t) / t$. Compute $y ' = v' y + v y' = v' / t - v / t^2$. Substituting back in to original equation gives us:
\[v' / t - v / t^2 + v / t^2 = 3 \cos{(2t)} \Rightarrow v' = 3t \cos{(2t)}\]
We can compute $\int t \cos{(2t)}$ by parts. Taking $u = t dv = \cos 2t, du = 1, v = 1/2 \sin 2t$ gives us
\[\int t \cos 2 t = \frac{1}{2} t \sin 2t  - \frac{1}{2} \int \sin 2t= \frac{t}{2}  \sin 2t  + \frac{1}{4}\cos{(2t)}.\]
Thus, $v =  \frac{3 t}{2}  \sin 2t  + \frac{3}{4}\cos{(2t)}+ C $ and the answer is
\[y = \frac{3 }{2}  \sin 2t  + \frac{3}{4t }\cos{(2t)}+ C /t  \]

\type{Integrating Factor}

\begin{ex} Solve $y' -2 y = t^2 e^{2 t  }$ by integrating factor.\end{ex}

Since this is already in the `right' form, we can immediately compute the integrating factor
\[u = e^{-\int2 dt } = e^{-2t}.\]

Therefore, 
\[ u x =\int uf + C  = \int t^2 e^{2t} e^{-2t} + c = \frac{1}{3} t^3 + C \Rightarrow x = e^{2t} \left( \frac{1}{3} t^3 + C \right)\]

\begin{ex}Solve  $y' + y / t = 3 \cos{(2t)}$ by integrating factor.\end{ex}

Compute the integrating factor $a = e^{\int 1/ t\ dt } = t$ and then write
\begin{align*} u x &= \int u f + C \\ t x &=  \int 3t \cos{(2t)} + C\end{align*} 
integrating by parts as in example \ref{vopint} gives us
\[x = \frac{3 }{2}  \sin 2t  + \frac{3}{4t }\cos{(2t)}+ \frac{C}{t}  \]



\subsection{Section 5 - Mixing Problems}

Mixing problems are a class of examples of differential equations involving mixing liquids. We assume `perfect mixing.' The most important equation is
\begin{align}\label{mixing} \frac{dx}{dt} = \mbox{Rate In} - \mbox{Rate Out} \end{align}
It's often helpful to look at the units and use `dimensional analysis' as sanity check.

\exs


\begin{ex}
A 50-gallon tank initially contains 20 gallons of pure water. Salt water solution with concentration of 1/2 lb/gal is added at a rate of 4 gal/min. A drain allows salt water to leave at 2 gal/min. How much salt is in the tank when it fills?
\end{ex}

Use equation \ref{mixing} (note: units should be lb/gal):
\[\frac{dx}{dt} = \mbox{Rate In} - \mbox{Rate Out}\]

First Rate in:
\[RI = \frac{1}{2} \frac{lb}{gal} \cdot 4 \frac{gal}{min} = 2 \frac{lb}{min}\]

For rate out we have:
\[RO = 2 \frac{gal}{min } \cdot \frac{x(t)}{v(t)} \frac{lb}{gal}\]
where $v(t) = 20 + 2t$ gives the volume of water in the tank as a function of time.

All together we have
\[\frac{dx}{dt} = 2 - \frac{x}{10 + t } \Leftrightarrow x' + \frac{1}{10 + t} x = 2\]
We can solve by integrating factor:
\[u = e^{\int \frac{1}{10 + t } dt } = 10 + t\]
\[(10 + t ) x = 2 \int (10 + t ) dt + C \Rightarrow x = \frac{t^2 + 20 t + C}{t + 10}\]

Using initial value $x(0) = 0$ (since we started with pure water) we get $C = 0$, and 
\[  x =   \frac{t(t  + 20)  }{t + 10}.\]
To find when the tank fills solve $50 = v(t) = 20  + 2 t  \Rightarrow t =15$. Substituting gives us $x(15) = 21$.




\subsection{Section 6 - Exact Differential Equations}


Consider a differential equation 
\[P dx + Q dy = 0\]
\begin{defn}[Exact]
We call such a differential equation \emph{exact} if 
\[\frac{\partial P }{\partial y} = \frac{\partial Q }{\partial x}.\]
\end{defn}
Given an exact differential equation there exists some $\Psi(x,y)$ with 
\[\frac{\partial \Psi}{\partial y} = Q, \frac{\partial \Psi}{\partial x} = P. \] 
Solutions to the ODE are then given implicity by $\Psi = c$.

Sometimes we're given an eqution which is not exact, but which can be transformed into an exact equation by multiplying by an integrating factor. 
There are a lot of poitential choices of integrating factor, and in general finding an integrating factor is as hard as solving the original equation. 
However, we have formulas for finding integrating factors which depend on only one variable.

\begin{re}[Integrating factor a funciton of $x$]
Compute
\[h = \frac{1}{Q} \left( \frac{\partial P }{ \partial y} - \frac{\partial Q}{ \partial x}\right).\]
If $h$ is a function of x alone then $\mu = e^{\int h dx}$ is an integrating factor.
\end{re}

\begin{re}[Integrating factor a funciton of $y$]
Compute
\[g = \frac{1}{P} \left( \frac{\partial P }{ \partial y} - \frac{\partial Q}{ \partial x}\right).\]
If $g$ is a function of x alone then $\mu = e^{-\int g dy}$ is an integrating factor.
\end{re}

ADD HOMOGENEOUS HERE!

\exs

\begin{ex} Is  the equation 
\[(y \cos x + 2 x e^y ) + ( \sin x + x^2 e^y -1) y' = 0 \]
exact? If so, solve.
\end{ex}

First we verify 
\[\frac{\partial P }{\partial y} = \cos x + 2x e^y =\frac{\partial Q }{\partial x},\]
so the equation is exact.

Now, we need to find a $\Psi$ with 
\[\frac{\partial \Psi}{\partial y} = Q,\quad \frac{\partial \Psi}{\partial x} = P. \] 

Thus integrate
\begin{align*}
\int \partial \Psi &= \int Q \partial y \\ 
\Psi &=  \int \sin x + x^2 e^y - 1 \partial y\\
&= y \sin x + x^2 e^y - y + h(x)
\end{align*}
for some unknown function $h$ of $x$. Of course, we can find $x$ by using the other equality:
\[\frac{\partial \Psi}{\partial x } = y \cos x + 2 x e^y + h'(x) =y \cos x + 2 x e^y = P .\]
So, $h'(x) = 0$ and $h(x) = C$ is a constant. Our solutions are therefore given implicity by 
\[ y \sin x + x^2 e^y - y = C.\]

\begin{ex} Solve the exact equation $(2x  + 3) + (2 y -2 ) y' = 0$. \end{ex}
$x^2 + 3x + y^2 - 2y = c$

\begin{ex} Solve the exact equation $(3x^2 - 2xy + 2)dx + (6y^2-x^2+3)dy =0$. \end{ex}
$x^3 - x^2 y + 2 x + 2 y ^3 + 3y = C $

\begin{ex} Is the following equation exact? $(x \log y + xy)dx + (y \log x + x y )dy =0$. \end{ex}
no


\begin{ex}Find $b$ such that the following equation is exact, then solve. $(x y ^2 + b x^2 y )dx + (x + y)x^2 dy = 0$ \end{ex}

$b = 3$ and $x^2 y ^2 + 2 x^3 y = C$

\type{Integrating Factor}

\begin{ex} Show that the following equation is not exact then solve using the integrating factor $\mu = 1 /xy^3$ 
\[x^2y^3 + x(1 + y^2) y' = 0 \]
\end{ex}

$x^2 + 2 \log |y | - y^{-2} = C $ and $y = 0$

\begin{ex}Find an integrating factor, and solve.
\[(3x^2 y + 2 x y + y^3)dx + (x^2 + y^2) dy =0\]
\end{ex}

$\mu = e^{3x}$ solution:$C=e^{3x}(3x^2 y + y^3)$


\begin{ex}Find an integrating factor, and solve.
\[y' = e^{2x} +y -1\]
\end{ex}

$\mu = e^{-x} $ and $y = C e^x + 1 + e ^{2x}$

\begin{ex}Solve using the integrating factor $\mu = e^{2x} / y$
\[y dx + (2 x y - e^{-2y}) dy = 0\]
\end{ex}

$y=0$ and $x e^{2 y} - \log y = C$

\type{Homogeneous}
ADD HOMOGENEOUS EXAMPLES

\subsection{Section 7 - Existence and Uniqueness of Solutions}
\begin{thm}[Existence]Consider the initial value problem
\[x' = f(t,x) \quad f(t_0) = x_0.\] 
If $f$ is defined and continuous near $(t_0, x_0)$ then a solution to the IVP exists, near $t_0$.
\end{thm}


\begin{thm}[Uniqueness]Consider the initial value problem
\[x' = f(t,x) \quad f(t_0) = x_0.\] 
If $f$ and $\frac{\partial f}{\partial x}$ are  defined and continuous near $(t_0, x_0)$ then a solution to the IVP exists and is unique, near $t_0$.
\end{thm}

\exs


\begin{ex}Show that the following both solve the IVP $x' = x^{1/3}; x(0) = 0$ 
\[x(t) = 0 \quad x(t) = 
\begin{cases}
(\frac{2}{3} t) ^{3/2} & t > 0 \\
0 & t \leq 0
\end{cases}\]
Why isn't the Uniqueness Theorem contradicted?
\end{ex}

First, compute (by chain rule) $x' = (2t/3)^{1/2} = x^{1/3}$ and $x' = 0 = x^{1/3}$. Next, note that $\frac{\partial f }{ \partial x} = 1 / x^{2/3}$ is not continuous at $x =0$, so the Uniqueness Theorem doesn't apply.

\begin{ex} Find the general solution to the following differential equation. Is there a solution with $y(0) = -3$? If not, why isn't the existence theorem contradicted?
\[t y' - y = t^2 \cos t\]\end{ex}
The general solution is (Integrating Factor) 
\[y = t \sin t + C t \]


\begin{ex}Show that $y(t) =0$ and $y(t) = t^3$ both solve $y' = 3 y^{2/3}$ with $y(0) =0$. Why doesn't this violate the uniqueness theorem?\end{ex}


\type{`Bounding Solutions'}

\begin{ex}[Exercise 2.7.29] Let $y$ be a solution to $y' = (y^2 -1) e^{ty}$ with $y(1) =0$. Prove that $-1 < y < 1$ for all $t$ where $y$ is defined.\end{ex}

First we're going to establish two facts:
\begin{enumerate}
\item $y(t) =1$ and $y(t) = -1$ are solutions to the differential equation
\item The uniqueness theorem applies along both of these solutions.
\end{enumerate}

Since the uniqueness theorem says that `solutions can't cross' and our solution starts between $1$ and $-1$ this is enough to show that our solution is always between $1$ and $-1$. You can think of these lines (shown in red below) as `fences' bounding our solution.

\[\includegraphics[scale=.7]{figures/{2.7.first}.pdf}\]

So now we just verify
\begin{enumerate}
\item If $y = 1$ we have $y' = 0$, so $0 = y' = (y^2 -1 ) e^{ty} =0 $. Similarly, if $y = -1$ we have $y' = 0$, so $0 = y' = (y^2 -1 ) e^{ty} =0 $.
\item $f = (y^2 -1) e^{ty}$ and $\frac{\partial f}{\partial y} = e^{t y} \left(2 y+t \left(-1+y^2\right)\right) $ are both continuous when $y = 1$ or $y = -1$ (in fact, they're continuous everywhere). Therefore, the uniqueness theorem applies.
\end{enumerate}



\begin{ex}[Exercise 2.7.31] Let $x$ be a solution to $x' = x - t ^2 + 2t$ with $x(0) = 1$. Prove that $x > t^2 $ for all $t$ where $x$ is defined.\end{ex}

As in the previous problem we're going to establish two facts:
\begin{enumerate}
\item  $x(t) = t^2$ is a  solution to the differential equation
\item The uniqueness theorem applies along this solution.
\end{enumerate}

Again remember that the uniqueness theorem says that `solutions can't cross.' Since our solution starts above $x(t) = t^2 $ this is enough to show that our solution is always above it. 

\[\includegraphics[scale=.7]{figures/{2.7.second}.pdf}\]

So now we just verify
\begin{enumerate}
\item If $x(t) = t^2$ we have $x'(t) = 2t$, so $x'(t) = 2t = t^2 - t^2  + 2t = x - t^2 + 2t  $, and $t^2$ satisifies our differential equation.
\item $f = x - t^2 + 2t$ and $\frac{\partial f}{\partial x} =1 $ are both continuous when $x = t^2$ or  (in fact, they're continuous everywhere). Therefore, the uniqueness theorem applies.
\end{enumerate}

\begin{ex}Consider the initial value problem
\[y' = \sqrt{y^2 + 1 } \ln(t+1) (y + \cos t ) + \sin t, \quad y(0) = 0\]
\begin{enumerate}
\item Do the theorems about the existence and uniqueness of solutions apply to this initial value problem? Explain.
\item Suppose $y(t)$ is a solution of the above initial value problem. Is it possible that $y(\pi) =0$? Why or why not? \\ (Hint: Note that $y' - \sin t = ( y + \cos t )'$.)
\end{enumerate}
\end{ex}
\begin{samepage}
\begin{enumerate}
\item Since the function is smooth (for $t > -1$), both uniqueness and existence theorems apply.
\item Using the hint, note that $y = -\cos t$ is a solution. Thus, by uniqueness theorem, it bounds $y$ below, and we can't have $y(\pi) = 0$.
\end{enumerate}


\[\includegraphics[scale=.7]{figures/{2.7.extra}.pdf}\]
\end{samepage}



\subsection{Section 7 - Autonomous Equations}

\begin{defn}[Autonomous] A differential equation of the form $$x' = f(x)$$ is called \emph{autonomous}.\end{defn}

\begin{defn}[Equilibrium] A point $x_0$ with $f(x_0)$ is called an \emph{equilibrium point}. The solution $f(t) = x_0$ is called an \emph{equilibrium solution}. \end{defn}	

\begin{defn}[Stable]An equilibrium point is called \emph{asymptotically stable} if solutions starting nearby stay near as $t \to infty$. More formally, if for every $\epsilon > 0$ ther eexists $\delta > 0$ such that solutions starting within $\delta$ of $x_0$ remain within $\epsilon$ for all $t$.\end{defn}


\begin{defn}[Unstable]An equilibrium point is called \emph{asymptotically unstable} if it is not stable.\end{defn}

\begin{defn}[Phase Line]A \emph{phase line} is just a plot of $f$ as a function of $x$.\end{defn}

\exs

\begin{ex}[Exercise 2.9.19]Plot the vector field, and phase line for $y' = 9 y - y^3$. Identify the equilibrium points and classify them:\end{ex}
\[\includegraphics[scale=.7]{figures/{2.9.19a}.pdf}\]
\[\includegraphics[scale=.7]{figures/{2.9.19b}.pdf}\]

\section{Chapter 4}

\subsection{Section ?? - Harmonic Motion}

\exs
\begin{ex}Suppose a particle of mass 1 is attached to a spring with spring constant 36, in a medium which imparts damping coefficient 2. Initial conditions $y(0) = 0$ and $y'(0) = \sqrt{35}$.  After what time is the particle guaranteed to be at most 1\% of it's maximum possible displacement?\end{ex}

Recall the formula
\[ m y'' + \mu y' + k y = f(t) \Leftrightarrow y'' + 2 y' + 36 y =0\]
So we can solve the characteristic equation:
\[\lambda^2 + 2 \lambda + 36 = 0 \quad \lambda = \frac{-2 \pm \sqrt{2^2 - 4 \cdot 36}}{2} = -1 \pm  i \sqrt{35}\]

Therefore, the general solution is just
\[y = e^{-t} ( C \sin{(t\sqrt{35})} + D \cos{(t\sqrt{35})} ).\]
for some constants $C,D$. Since we have initial conditions $y(0) = 0$ and $y'(0) = \sqrt{35}$ we solve to find $D = 0$, $C = 1$. 

Now let's transform equation using the usual formulae
\[y = A e^{\alpha t}  \cos{(\omega t - \phi)} \quad A^2 = 0^2 + 1^2 , 
\phi = \tan^{-1}(1/0)\]
of course, this value of $\phi$ doesn't really make sense, but in the limit, we have $\phi = \pi/ 2$. We have now
\[ y =  e^{ -t} \cos{(\sqrt{35} t - \pi /2)}\]
so we see that the max possible displacement is 1, and if $t > - \ln .01 \sim 4.605170$ we must have $y$ at most $.01$.


\end{document}
