\documentclass[11pt]{article} 



\makeatletter
\renewcommand\section{\@startsection{section}{1}{\z@}%
                                  {-3.5ex \@plus -1ex \@minus -.2ex}%
                                  {2.3ex \@plus.2ex}%
                                  {\normalfont\large\bfseries}}
\makeatother

\addtolength{\oddsidemargin}{-.875in}
\addtolength{\evensidemargin}{-.875in}
\addtolength{\textwidth}{1.75in}
\addtolength{\topmargin}{-.875in}
\addtolength{\textheight}{1.75in}


\usepackage{amssymb}
\usepackage{amsmath}
\usepackage{amsthm}
\usepackage{graphicx,caption,subcaption}


\usepackage{titling}
\setlength{\droptitle}{-6em}
\posttitle{\par\end{center}\vspace{-4.8em}}

\newcommand{\R}{{\ensuremath{\mathbb{R}}} }
\newcommand{\Q}{{\ensuremath{\mathbb{Q}}} }
\newcommand{\C}{{\ensuremath{\mathbb{C}}} }
\newcommand{\N}{{\ensuremath{\mathbb{N}}} }
\newcommand{\Z}{{\ensuremath{\mathbb{Z}}} }

\newcommand{\sexion}{\addtocounter{section}{1} }


\newcommand{\hint}[1]{{(\emph{Hint:} #1)}} %This line shows hints
%\newcommand{\hint}[1]{} %Use this line to hide all hints


\usepackage{fancyhdr}
\pagestyle{fancyplain}
\renewcommand{\headrulewidth}{0pt}

\begin{document}

%\lhead{}
\rhead{Forced Harmonic Motion}
\section{Problem}
\[ x'' + 4 x' + 5 x = \tan x\]

\section{Solution}

First we need to find two linearly independent solutions to the associated homogeneous equation
\[x'' + 4 x' + 5 x =0 \quad\rightarrow\quad \lambda^2 + 4 \lambda + 5 =0 \Rightarrow \lambda = \frac{-4 \pm \sqrt{4^2 -4 \cdot 5}}{2} = -2 \pm i\]
So we have $x_1(t) = e^{-2 t} \cos{t}$ and $x_1(t) = e^{-2 t} \sin{t}$.

Now we need a particular solution $x_p(t)$ to the original equation. Since $g(t) = \tan x$ we can't use undetermined coefficient, and are forced to use variation of parameter.

So let's compute the Wronskian,
\begin{align*} W &= \left| \begin{array}{cc}  e^{-2 t} \cos{t} & e^{-2 t} \sin{t} \\ -2 e^{-2 t} \cos{t}-e^{-2 t} \sin{t} &  e^{-2 t} \cos{t}-2 e^{-2 t} \sin{t} \end{array}\right| \\ &= e^{-4 t} \left( \cos{t}(\cos{t} - 2 \sin{t}) - \sin{t} (-2 \cos{t} -  \sin{t}) \right) \\ &= e^{-4t}   \end{align*}

Now recall that variation of parameter tells us that $x_p = v_1(t) x_1(t) + v_2(t) x_2(t)$ for
\[v'_2 = \frac{x_1 \cdot g}{W} \quad v'_1 = - \frac{x_2 \cdot g }{W}\]
so all that remains is to compute 
\begin{align*} v_2 &= \int  \frac{x_1 \cdot g}{W}\\ &= \int \frac{e^{-2t} \cos t\cdot \tan t}{e^{-4t}} \\ &= \int e^{2t} \sin t \end{align*}
Recall
\[ \sin t = \frac{ e^{i t} - e^{-i t}}{2 i} \quad \cos t = \frac{e^{it} + e^{-it} }{2} \quad \tan t = -\frac{i \left(-1+e^{2 i t}\right)}{1+e^{2 i t}} \]
\end{document}
