\documentclass[11pt]{article} 



\makeatletter
\renewcommand\section{\@startsection{section}{1}{\z@}%
                                  {-3.5ex \@plus -1ex \@minus -.2ex}%
                                  {2.3ex \@plus.2ex}%
                                  {\normalfont\large\bfseries}}
\makeatother

\addtolength{\oddsidemargin}{-.875in}
\addtolength{\evensidemargin}{-.875in}
\addtolength{\textwidth}{1.75in}
\addtolength{\topmargin}{-.875in}
\addtolength{\textheight}{1.75in}


\usepackage{amssymb}
\usepackage{amsmath}
\usepackage{amsthm}
\usepackage{graphicx,caption,subcaption}


\usepackage{titling}
\setlength{\droptitle}{-6em}
\posttitle{\par\end{center}\vspace{-4.8em}}

\newcommand{\R}{{\ensuremath{\mathbb{R}}} }
\newcommand{\Q}{{\ensuremath{\mathbb{Q}}} }
\newcommand{\C}{{\ensuremath{\mathbb{C}}} }
\newcommand{\N}{{\ensuremath{\mathbb{N}}} }
\newcommand{\Z}{{\ensuremath{\mathbb{Z}}} }

\newcommand{\sexion}{\addtocounter{section}{1} }


\newcommand{\hint}[1]{{(\emph{Hint:} #1)}} %This line shows hints
%\newcommand{\hint}[1]{} %Use this line to hide all hints


\usepackage{fancyhdr}
\pagestyle{fancyplain}
\renewcommand{\headrulewidth}{0pt}

\begin{document}

%\lhead{}
\rhead{Reduction of Order}
\section{Problem}

\begin{equation}\label{prob}t^2 y'' + 3t y' - 3y = 0\end{equation}
\begin{enumerate}
\item Check that $y_1(t) = t$ is a solution
\item Find the general solution
\end{enumerate}

\section{Solution}
For part one, we just compute
\[y(t) = t \quad y'(t) =1 \quad y''(t) = 0\]
and plug in to \ref{prob} to get
\[t^2 (0) + 3t ( 1) - 3 (t) = 0\]

For part 2, guess a solution of the form
\[y_2 = v(t) y_1 = t v(t) \quad y_2' = t v' + v \quad y_2'' = t v'' + 2v'\]
Plugging in to \ref{prob} we get
\begin{align*}t^2( t v'' + 2v')  + 3t ( t v' + v) - 3 (t v) &= t^3v'' + 2 t^2 v' + 3t^2 v' + 3t v - 3tv \\ &= t^3 v'' + 5t^2 v'  \end{align*}
If we let $u = v' $ we have 
\[0= t^3 u' + 5 t^2 u\]
or
\[-\frac{5}{t} dt   = \frac{1}{u} du\]
integrating\
\[-5 \ln t = \ln u +C\]
\[u = C t^{-5}\]
But, since we put $u = v'$ 
\[v = C \int t^{-5} = C \left( -  \frac{1}{4} t^{-4} + D\right) \sim C (t ^{-4} +D )\]
and 
\[y_2(t) = C(t^{-4} + D ) \cdot t = Ct^{-3}+  Dt \]
solves \ref{prob} regardless of $C,D$. Since there are two degrees of freedom in this solution, it is in fact the general solution. Note that it includes $y_1$ as ($C=0, D=1$).
\end{document}
